src/Imps/Imp/Bigstep.v
@@ -7,8 +7,7 @@ Inductive AEval : AExp -> State -> nat -> Prop :=
 | EvalVar :
     forall (v : Loc) (s : State), AEval (Var v) s (s v)
 | EvalABinOp :
-    forall (f : nat -> nat -> nat)
-           (a1 a2 : AExp) (s : State) (n1 n2 : nat),
+    forall (f : nat -> nat -> nat) (a1 a2 : AExp) (s : State) (n1 n2 : nat),
       AEval a1 s n1 -> AEval a2 s n2 ->
         AEval (ABinOp f a1 a2) s (f n1 n2).
 
@@ -18,10 +17,9 @@ Lemma AEval_det :
   forall {a : AExp} {s : State} {n m : nat},
     AEval a s n -> AEval a s m -> n = m.
 Proof.
-  intros a s n m H. revert m.
-  induction H; inversion 1; subst; clear H.
-    1-2: reflexivity.
-    rewrite (IHAEval1 _ H7), (IHAEval2 _ H8). reflexivity.
+  intros a s n m H; revert m.
+  induction H; inversion 1; subst; clear H; [easy.. |].
+  now rewrite (IHAEval1 _ H7), (IHAEval2 _ H8).
 Qed.
 
 #[global] Hint Resolve in_or_app : core.
@@ -33,7 +31,7 @@ Lemma AEval_acompatible :
         AEval a s2 n.
 Proof.
   unfold acompatible.
-  induction 1; cbn in *; intros; try rewrite H; auto 6.
+  now induction 1; cbn in *; intros; try rewrite H; auto 6.
 Qed.
 
 Lemma AEval_acompatible_det :
@@ -45,25 +43,24 @@ Lemma AEval_acompatible_det :
         n1 = n2.
 Proof.
   induction 1; cbn; intros; auto.
-    inv H.
-    inv H.
-    inv H1. erewrite IHAEval1, IHAEval2; eauto.
+  - inv H.
+  - inv H.
+  - inv H1.
+    now erewrite IHAEval1, IHAEval2; eauto.
 Qed.
 
 Inductive BEval : BExp -> State -> bool -> Prop :=
 | EvalBConst :
     forall (s : State) (b : bool), BEval (BConst b) s b
 | BEval_BRelOp :
-    forall (f : nat -> nat -> bool)
-           (a1 a2 : AExp) (s : State) (n1 n2 : nat),
+    forall (f : nat -> nat -> bool) (a1 a2 : AExp) (s : State) (n1 n2 : nat),
       AEval a1 s n1 -> AEval a2 s n2 ->
         BEval (BRelOp f a1 a2) s (f n1 n2)
 | EvalNot :
     forall (e : BExp) (s : State) (b : bool),
       BEval e s b -> BEval (Not e) s (negb b)
 | BEval_BBinOp :
-    forall (f : bool -> bool -> bool)
-           (e1 e2 : BExp) (s : State) (b1 b2 : bool),
+    forall (f : bool -> bool -> bool) (e1 e2 : BExp) (s : State) (b1 b2 : bool),
       BEval e1 s b1 -> BEval e2 s b2 ->
         BEval (BBinOp f e1 e2) s (f b1 b2).
 
@@ -74,10 +71,13 @@ Lemma BEval_det :
     BEval e s b1 -> forall {b2 : bool}, BEval e s b2 -> b1 = b2.
 Proof.
   induction 1; intros.
-    inv H.
-    inv H1. rewrite (AEval_det H H7), (AEval_det H0 H8). reflexivity.
-    inv H0. rewrite (IHBEval _ H2). reflexivity.
-    inv H1. rewrite (IHBEval1 _ H7), (IHBEval2 _ H8). reflexivity.
+  - inv H.
+  - inv H1.
+    now rewrite (AEval_det H H7), (AEval_det H0 H8).
+  - inv H0.
+    now rewrite (IHBEval _ H2).
+  - inv H1.
+    now rewrite (IHBEval1 _ H7), (IHBEval2 _ H8).
 Qed.
 
 #[global] Hint Resolve AEval_acompatible : core.
@@ -89,7 +89,7 @@ Lemma BEval_bcompatible :
       bcompatible e s1 s2 -> BEval e s2 b.
 Proof.
   unfold bcompatible.
-  induction 1; cbn in *; intros; constructor; eauto 6.
+  now induction 1; cbn in *; intros; constructor; eauto 6.
 Qed.
 
 Lemma BEval_bcompatible_det :
@@ -99,9 +99,8 @@ Lemma BEval_bcompatible_det :
       bcompatible e s1 s2 -> b1 = b2.
 Proof.
   intros.
-  assert (BEval e s2 b1).
-    eapply BEval_bcompatible; eauto.
-  eapply BEval_det; eauto.
+  assert (BEval e s2 b1) by (eapply BEval_bcompatible; eauto).
+  now eapply BEval_det; eauto.
 Qed.
 
 Inductive CEval : Com -> State -> State -> Prop :=
@@ -135,8 +134,8 @@ Example while_true_do_skip :
     ~ CEval (While (BConst true) Skip) s1 s2.
 Proof.
   intros s1 s2 H.
-  remember (While (BConst true) Skip) as w. revert Heqw.
-  induction H; intros; inv Heqw. inv H.
+  remember (While (BConst true) Skip) as w; revert Heqw.
+  now induction H; intros; inv Heqw.
 Qed.
 
 #[global] Hint Rewrite @AEval_det : core.
@@ -146,18 +145,18 @@ Lemma CEval_det :
   forall (c : Com) (s s1 : State),
     CEval c s s1 -> forall s2 : State, CEval c s s2 -> s1 = s2.
 Proof.
-  induction 1; intros;
-  match goal with
-  | H : CEval ?c _ _ |- _ => is_var c + inv H
-  end;
-  repeat match goal with
-  | IH : forall _, CEval _ _ _ -> _, H : CEval _ _ _ |- _ =>
-      let H' := fresh "H" in
-        assert (H' := IH _ H); clear H; rename H' into H; subst
-  | H : BEval ?b ?s _, H' : BEval ?b ?s _ |- _ =>
-      let H'' := fresh "H" in
-        assert (H'' := BEval_det H H'); clear H H'
-  end; eauto; try congruence.
+  now induction 1; intros;
+    match goal with
+    | H : CEval ?c _ _ |- _ => is_var c + inv H
+    end;
+    repeat match goal with
+    | IH : forall _, CEval _ _ _ -> _, H : CEval _ _ _ |- _ =>
+        let H' := fresh "H" in
+          assert (H' := IH _ H); clear H; rename H' into H; subst
+    | H : BEval ?b ?s _, H' : BEval ?b ?s _ |- _ =>
+        let H'' := fresh "H" in
+          assert (H'' := BEval_det H H'); clear H H'
+    end; eauto; try congruence.
 Qed.
 
 (** * Equivalence of big step and denotational semantics *)
@@ -166,14 +165,14 @@ Lemma AEval_aeval :
   forall {a : AExp} {s : State} {n : nat},
     AEval a s n -> aeval s a = n.
 Proof.
-  induction 1; cbn; rewrite ?IHAEval1, ?IHAEval2; reflexivity.
+  now induction 1; cbn; rewrite ?IHAEval1, ?IHAEval2.
 Qed.
 
 Lemma aeval_AEval :
   forall {a : AExp} {s : State} {n : nat},
     aeval s a = n -> AEval a s n.
 Proof.
-  induction a; cbn; intros; rewrite <- H; auto.
+  now induction a; cbn; intros; rewrite <- H; auto.
 Qed.
 
 Lemma BEval_beval :
@@ -181,10 +180,10 @@ Lemma BEval_beval :
     BEval e s b -> beval s e = b.
 Proof.
   induction 1; cbn.
-    reflexivity.
-    rewrite (AEval_aeval H), (AEval_aeval H0). reflexivity.
-    rewrite IHBEval. reflexivity.
-    rewrite IHBEval1, IHBEval2. reflexivity.
+  - easy.
+  - now rewrite (AEval_aeval H), (AEval_aeval H0).
+  - now rewrite IHBEval.
+  - now rewrite IHBEval1, IHBEval2.
 Qed.
 
 Lemma beval_BEval :
@@ -192,7 +191,7 @@ Lemma beval_BEval :
     beval s e = b -> BEval e s b.
 Proof.
   induction e; cbn; intros; subst; auto.
-    constructor; apply aeval_AEval; reflexivity.
+  now constructor; apply aeval_AEval.
 Qed.
 
 #[global] Hint Immediate aeval_AEval beval_BEval : core.
@@ -201,7 +200,8 @@ Lemma ceval_CEval :
   forall (n : nat) (c : Com) (s1 s2 : State),
     ceval n c s1 = Some s2 -> CEval c s1 s2.
 Proof.
-  intros n c s1. functional induction ceval n c s1; intros; inv H; eauto.
+  intros n c s1.
+  now functional induction ceval n c s1; intros; inv H; eauto.
 Qed.
 
 Lemma CEval_ceval :
@@ -209,20 +209,25 @@ Lemma CEval_ceval :
     CEval c s1 s2 -> exists n : nat, ceval n c s1 = Some s2.
 Proof.
   induction 1.
-    exists 1. cbn. reflexivity.
-    exists 1. cbn. do 2 f_equal. apply AEval_aeval. assumption.
-    destruct IHCEval1 as [n1 IH1], IHCEval2 as [n2 IH2].
-      exists (S (n1 + n2)). (* Should be S (max n1 n2) *)
-      cbn. rewrite (ceval_plus n1 n2 _ _ _ IH1), Nat.add_comm.
-        apply ceval_plus. assumption.
-    destruct IHCEval as [n IH]. exists (S n). cbn.
-      apply BEval_beval in H. rewrite H. assumption.
-    destruct IHCEval as [n IH]. exists (S n). cbn.
-      apply BEval_beval in H. rewrite H. assumption.
-    exists 1. cbn. apply BEval_beval in H. rewrite H. reflexivity.
-    destruct IHCEval1 as [n1 IH1], IHCEval2 as [n2 IH2].
-      exists (S (n1 + n2)). cbn. (* Should be S (max n1 n2) *)
-      apply BEval_beval in H. rewrite H.
-      rewrite (ceval_plus _ _ _ _ _ IH1), Nat.add_comm.
-      apply ceval_plus. assumption.
+  - now exists 1; cbn.
+  - exists 1; cbn.
+    do 2 f_equal.
+    now apply AEval_aeval.
+  - destruct IHCEval1 as [n1 IH1], IHCEval2 as [n2 IH2].
+    exists (S (n1 + n2)); cbn. (* Should be S (max n1 n2) *)
+    rewrite (ceval_plus n1 n2 _ _ _ IH1), Nat.add_comm.
+    now apply ceval_plus.
+  - destruct IHCEval as [n IH].
+    exists (S n); cbn.
+    now apply BEval_beval in H as ->.
+  - destruct IHCEval as [n IH].
+    exists (S n); cbn.
+    now apply BEval_beval in H as ->.
+  - exists 1; cbn.
+    now apply BEval_beval in H as ->.
+  - destruct IHCEval1 as [n1 IH1], IHCEval2 as [n2 IH2].
+    exists (S (n1 + n2)); cbn. (* Should be S (max n1 n2) *)
+    apply BEval_beval in H as ->.
+    rewrite (ceval_plus _ _ _ _ _ IH1), Nat.add_comm.
+    now apply ceval_plus.
 Qed.
