src/Imps/Imp/SmallstepWithContexts.v
@@ -31,15 +31,12 @@ Inductive AEval (s : State) : AExp -> AExp -> Prop :=
 
 #[global] Hint Constructors AStep AEval : core.
 
-(*
 Function AExp_to_AContext (a : AExp) : AContext * AExp :=
 match a with
 | AConst n => (AC_Var, AConst n)
 | Var x => (AC_Var, Var x)
-| ABinOp f (AConst n) a2 =>
-        let '(G, a) := AExp_to_AContext a2 in (AC_R f n G, a)
-| ABinOp f a1 a2 =>
-        let '(G, a) := AExp_to_AContext a1 in (AC_L f G a2, a)
+| ABinOp f (AConst n) a2 => let '(G, a) := AExp_to_AContext a2 in (AC_R f n G, a)
+| ABinOp f a1 a2 => let '(G, a) := AExp_to_AContext a1 in (AC_L f G a2, a)
 end.
 
 Lemma AExp_to_AContext_aput :
@@ -47,8 +44,7 @@ Lemma AExp_to_AContext_aput :
     AExp_to_AContext a1 = (G, a2) -> aput G a2 = a1.
 Proof.
   intros a1.
-  functional induction AExp_to_AContext a1;
-    intros; inv H; cbn; f_equal; auto.
+  now functional induction AExp_to_AContext a1; intros; inv H; cbn; f_equal; auto.
 Qed.
 
 Lemma AExp_to_AContext_aput' :
@@ -56,39 +52,38 @@ Lemma AExp_to_AContext_aput' :
     aput (fst (AExp_to_AContext a)) (snd (AExp_to_AContext a)) = a.
 Proof.
   intros. apply AExp_to_AContext_aput.
-  destruct AExp_to_AContext. cbn. reflexivity.
+  now destruct AExp_to_AContext; cbn.
 Qed.
-*)
 
 Lemma AEval_Smallstep_AEval :
   forall (s : State) (a1 a2 : AExp),
     AEval s a1 a2 <-> Smallstep.AEval s a1 a2.
 Proof.
   split.
-    intro. inv H. induction G; cbn; auto. induction H0; auto.
-    induction 1.
-      change (Var x)
+  - intro. inv H. induction G; cbn; auto. induction H0; auto.
+  - induction 1.
+    + change (Var x)
         with (aput AC_Var (Var x));
       change (AConst (s x))
         with (aput AC_Var (AConst (s x))).
-        constructor. constructor.
-      inv IHAEval.
-        change (ABinOp f (aput G a0) a2)
-          with (aput (AC_L f G a2) a0).
-        change (ABinOp f (aput G a3) a2)
-          with (aput (AC_L f G a2) a3).
-        constructor. assumption.
-      inv IHAEval.
-        change (ABinOp f (AConst n) (aput G a1))
-          with (aput (AC_R f n G) a1).
-        change (ABinOp f (AConst n) (aput G a0))
-          with (aput (AC_R f n G) a0).
-        constructor. assumption.
-      change (ABinOp f (AConst n1) (AConst n2))
+      do 2 constructor.
+    + inv IHAEval.
+      change (ABinOp f (aput G a0) a2)
+        with (aput (AC_L f G a2) a0).
+      change (ABinOp f (aput G a3) a2)
+        with (aput (AC_L f G a2) a3).
+      now constructor.
+    + inv IHAEval.
+      change (ABinOp f (AConst n) (aput G a1))
+        with (aput (AC_R f n G) a1).
+      change (ABinOp f (AConst n) (aput G a0))
+        with (aput (AC_R f n G) a0).
+      now constructor.
+    + change (ABinOp f (AConst n1) (AConst n2))
         with (aput AC_Var (ABinOp f (AConst n1) (AConst n2)));
       change (AConst (f n1 n2))
         with (aput AC_Var (AConst (f n1 n2))).
-        constructor. constructor.
+      now constructor.
 Qed.
 
 Inductive BStep : BExp -> BExp -> Prop :=
@@ -103,10 +98,6 @@ Inductive BStep : BExp -> BExp -> Prop :=
 
 Inductive BContext : Type :=
 | BC_Hole : BContext
-(*
-| BC_BRelOp_L : (nat -> nat -> bool) -> BContext -> AExp -> BContext
-| BC_BRelOp_R : (nat -> nat -> bool) -> nat -> BContext -> BContext
-*)
 | BC_Not : BContext -> BContext
 | BC_BBinOp_L : (bool -> bool -> bool) -> BContext -> BExp -> BContext
 | BC_BBinOp_R : (bool -> bool -> bool) -> bool -> BContext -> BContext.
@@ -114,10 +105,6 @@ Inductive BContext : Type :=
 Fixpoint bput (G : BContext) (e : BExp) : BExp :=
 match G with
 | BC_Hole => e
-(*
-| BC_BRelOp_L f G' a => BRelOp f (bput G' e) a
-| BC_BRelOp_R f n G' => BRelOp f (AConst n) (bput G' e)
-*)
 | BC_Not G' => Not (bput G' e)
 | BC_BBinOp_L f G' e' => BBinOp f (bput G' e) e'
 | BC_BBinOp_R f b G' => BBinOp f (BConst b) (bput G' e)
@@ -133,51 +120,39 @@ Lemma BEval_Smallstep_BEval :
     BEval b1 b2 <-> Smallstep.BEval s b1 b2.
 Proof.
   split.
-    intro. inv H. induction G; cbn; auto. inv H0; auto.
-    induction 1.
-      admit.
-      admit.
-      {
-        change (BRelOp f (AConst n1) (AConst n2))
-          with (bput BC_Hole (BRelOp f (AConst n1) (AConst n2))).
-        change (BConst (f n1 n2 ))
-          with (bput BC_Hole (BConst (f n1 n2))).
-        constructor. constructor.
-      }
-      {
-        inv IHBEval.
-        change (Not (bput G b1)) with (bput (BC_Not G) b1).
-        change (Not (bput G b2)) with (bput (BC_Not G) b2).
-        constructor. assumption.
-      }
-      {
-        change (Not (BConst b))
-          with (bput BC_Hole (Not (BConst b))).
-        change (BConst (negb b))
-          with (bput BC_Hole (BConst (negb b))).
-        constructor. constructor.
-      }
-      {
-        inv IHBEval.
-        change (BBinOp f (bput G b1) e2)
-          with (bput (BC_BBinOp_L f G e2) b1).
-        change (BBinOp f (bput G b2) e2)
-          with (bput (BC_BBinOp_L f G e2) b2).
-        constructor. assumption.
-      }
-      {
-        inv IHBEval.
-        change (BBinOp f (BConst b) (bput G b1))
-          with (bput (BC_BBinOp_R f b G) b1).
-        change (BBinOp f (BConst b) (bput G b2))
-          with (bput (BC_BBinOp_R f b G) b2).
-        constructor. assumption.
-      }
-      {
-        change (BBinOp f (BConst b1) (BConst b2))
-          with (bput BC_Hole (BBinOp f (BConst b1) (BConst b2))).
-        change (BConst (f b1 b2))
-          with (bput BC_Hole (BConst (f b1 b2))).
-        constructor. constructor.
-      }
+  - intro. inv H. induction G; cbn; auto. inv H0; auto.
+  - induction 1.
+    + admit.
+    + admit.
+    + change (BRelOp f (AConst n1) (AConst n2))
+        with (bput BC_Hole (BRelOp f (AConst n1) (AConst n2))).
+      change (BConst (f n1 n2 ))
+        with (bput BC_Hole (BConst (f n1 n2))).
+      now do 2 constructor.
+    + inv IHBEval.
+      change (Not (bput G b1)) with (bput (BC_Not G) b1).
+      change (Not (bput G b2)) with (bput (BC_Not G) b2).
+      now constructor.
+    + change (Not (BConst b))
+        with (bput BC_Hole (Not (BConst b))).
+      change (BConst (negb b))
+        with (bput BC_Hole (BConst (negb b))).
+      now do 2 constructor.
+    + inv IHBEval.
+      change (BBinOp f (bput G b1) e2)
+        with (bput (BC_BBinOp_L f G e2) b1).
+      change (BBinOp f (bput G b2) e2)
+        with (bput (BC_BBinOp_L f G e2) b2).
+      now constructor.
+    + inv IHBEval.
+      change (BBinOp f (BConst b) (bput G b1))
+        with (bput (BC_BBinOp_R f b G) b1).
+      change (BBinOp f (BConst b) (bput G b2))
+        with (bput (BC_BBinOp_R f b G) b2).
+      now constructor.
+    + change (BBinOp f (BConst b1) (BConst b2))
+        with (bput BC_Hole (BBinOp f (BConst b1) (BConst b2))).
+      change (BConst (f b1 b2))
+        with (bput BC_Hole (BConst (f b1 b2))).
+      now do 2 constructor.
 Admitted.
