src/Imps/Imp/Denotational.v
@@ -43,17 +43,14 @@ Lemma ceval_plus :
   forall (n k : nat) (c : Com) (s1 s2 : State),
     ceval n c s1 = Some s2 -> ceval (n + k) c s1 = Some s2.
 Proof.
-  induction n as [| n']; cbn; intros.
-    inv H.
-    destruct c; auto.
-      destruct (ceval n' c1 s1) eqn: Heq.
-        erewrite IHn'; eauto.
-        inv H.
-      destruct (beval s1 b) eqn: Hb; eauto.
-      destruct (beval s1 b) eqn: Hb; eauto.
-        destruct (ceval n' c s1) eqn: Heq.
-          erewrite IHn'; eauto.
-          inv H.
+  induction n as [| n']; cbn; intros; [easy |].
+  destruct c; auto.
+  - destruct (ceval n' c1 s1) eqn: Heq; [| easy].
+    now erewrite IHn'; eauto.
+  - destruct (beval s1 b) eqn: Hb; eauto.
+  - destruct (beval s1 b) eqn: Hb; [| easy].
+    destruct (ceval n' c s1) eqn: Heq; [| easy].
+    now erewrite IHn'; eauto.
 Qed.
 
 Lemma ceval_plus' :
@@ -61,5 +58,7 @@ Lemma ceval_plus' :
     ceval n c s1 = Some s2 ->
       forall k : nat, ceval (k + n) c s1 = Some s2.
 Proof.
-  intros. rewrite Nat.add_comm. apply ceval_plus. assumption.
+  intros.
+  rewrite Nat.add_comm.
+  now apply ceval_plus.
 Qed.
