src/Imps/Imp/SmallstepBigstep.v
@@ -6,18 +6,22 @@ Lemma Bigstep_Smallstep_AExp :
   forall (s : State) (a : AExp) (n : nat),
     Bigstep.AEval a s n <-> Smallstep.AEvals s a (AConst n).
 Proof.
-  split; intro.
-    apply Bigstep.AEval_aeval in H. apply Smallstep.aeval_AEvals. assumption.
-    apply Smallstep.AEvals_aeval in H. apply Bigstep.aeval_AEval. assumption.
+  split; intros.
+  - apply Bigstep.AEval_aeval in H.
+    now apply Smallstep.aeval_AEvals.
+  - apply Smallstep.AEvals_aeval in H.
+    now apply Bigstep.aeval_AEval.
 Qed.
 
 Lemma Bigstep_Smallstep_BExp :
   forall (s : State) (e : BExp) (b : bool),
     Bigstep.BEval e s b <-> Smallstep.BEvals s e (BConst b).
 Proof.
-  split; intro.
-    apply Bigstep.BEval_beval in H. apply Smallstep.beval_BEvals. assumption.
-    apply Smallstep.BEvals_beval in H. apply Bigstep.beval_BEval. assumption.
+  split; intros.
+  - apply Bigstep.BEval_beval in H.
+    now apply Smallstep.beval_BEvals.
+  - apply Smallstep.BEvals_beval in H.
+    now apply Bigstep.beval_BEval.
 Qed.
 
 Lemma Bigstep_Smallstep_Com :
@@ -25,8 +29,8 @@ Lemma Bigstep_Smallstep_Com :
     Bigstep.CEval c s1 s2 <-> Smallstep.CEvals (c, s1) (Skip, s2).
 Proof.
   split; intro.
-    apply Bigstep.CEval_ceval in H. destruct H as [n H].
-      eapply Smallstep.ceval_CEvals. eassumption.
-    apply Smallstep.CEvals_ceval in H. destruct H as [n H].
-      apply Bigstep.ceval_CEval with n. assumption.
+  - apply Bigstep.CEval_ceval in H as [n H].
+    now apply Smallstep.ceval_CEvals in H.
+  - apply Smallstep.CEvals_ceval in H as [n H].
+    now apply Bigstep.ceval_CEval with n.
 Qed.
