src/Imps/Imp_resultis.v
@@ -113,28 +113,28 @@ with CEval_det :
   forall (c : Com) (s s1 : State),
     CEval c s s1 -> forall s2 : State, CEval c s s2 -> s1 = s2.
 Proof.
-  destruct 1; intros * HI *; inv HI.
-    rewrite (AEval_det _ _ _ _ H H3), (AEval_det _ _ _ _ H0 H6). reflexivity.
-    rewrite (AEval_det _ _ _ _ H H3), (AEval_det _ _ _ _ H0 H6). reflexivity.
-    rewrite (AEval_det _ _ _ _ H H3), (AEval_det _ _ _ _ H0 H6). reflexivity.
-    specialize (CEval_det _ _ _ H _ H3). subst.
-      rewrite (AEval_det _ _ _ _ H0 H6). reflexivity.
-  destruct 1; intros * HI *; inv HI.
-    rewrite (AEval_det _ _ _ _ H H3), (AEval_det _ _ _ _ H0 H6). reflexivity.
-    rewrite (AEval_det _ _ _ _ H H3), (AEval_det _ _ _ _ H0 H6). reflexivity.
-    rewrite (BEval_det _ _ _ H _ H1). reflexivity.
-    rewrite (BEval_det _ _ _ H _ H3), (BEval_det _ _ _ H0 _ H6). reflexivity.
-    rewrite (BEval_det _ _ _ H _ H3), (BEval_det _ _ _ H0 _ H6). reflexivity.
-  destruct 1; intros * HI *; inv HI.
-    rewrite (AEval_det _ _ _ _ H H4). reflexivity.
-    destruct (CEval_det _ _ _ H _ H3), (CEval_det _ _ _ H0 _ H6). reflexivity.
-    rewrite (CEval_det _ _ _ H0 _ H7). reflexivity.
-    specialize (BEval_det _ _ _ H _ H6). congruence.
-    specialize (BEval_det _ _ _ H _ H6). congruence.
-    rewrite (CEval_det _ _ _ H0 _ H7). reflexivity.
-    specialize (BEval_det _ _ _ H _ H2). congruence.
-    specialize (BEval_det _ _ _ H _ H6). congruence.
-    destruct (CEval_det _ _ _ H0 _ H5), (CEval_det _ _ _ H1 _ H8). reflexivity.
+  - destruct 1; intros * HI *; inv HI.
+    + rewrite (AEval_det _ _ _ _ H H3), (AEval_det _ _ _ _ H0 H6). reflexivity.
+    + rewrite (AEval_det _ _ _ _ H H3), (AEval_det _ _ _ _ H0 H6). reflexivity.
+    + rewrite (AEval_det _ _ _ _ H H3), (AEval_det _ _ _ _ H0 H6). reflexivity.
+    + specialize (CEval_det _ _ _ H _ H3). subst.
+       rewrite (AEval_det _ _ _ _ H0 H6). reflexivity.
+  - destruct 1; intros * HI *; inv HI.
+    + rewrite (AEval_det _ _ _ _ H H3), (AEval_det _ _ _ _ H0 H6). reflexivity.
+    + rewrite (AEval_det _ _ _ _ H H3), (AEval_det _ _ _ _ H0 H6). reflexivity.
+    + rewrite (BEval_det _ _ _ H _ H1). reflexivity.
+    + rewrite (BEval_det _ _ _ H _ H3), (BEval_det _ _ _ H0 _ H6). reflexivity.
+    + rewrite (BEval_det _ _ _ H _ H3), (BEval_det _ _ _ H0 _ H6). reflexivity.
+  - destruct 1; intros * HI *; inv HI.
+    + rewrite (AEval_det _ _ _ _ H H4). reflexivity.
+    + destruct (CEval_det _ _ _ H _ H3), (CEval_det _ _ _ H0 _ H6). reflexivity.
+    + rewrite (CEval_det _ _ _ H0 _ H7). reflexivity.
+    + specialize (BEval_det _ _ _ H _ H6). congruence.
+    + specialize (BEval_det _ _ _ H _ H6). congruence.
+    + rewrite (CEval_det _ _ _ H0 _ H7). reflexivity.
+    + specialize (BEval_det _ _ _ H _ H2). congruence.
+    + specialize (BEval_det _ _ _ H _ H6). congruence.
+    + destruct (CEval_det _ _ _ H0 _ H5), (CEval_det _ _ _ H1 _ H8). reflexivity.
 Qed.
 
 Set Warnings "-funind-cannot-define-graph".
@@ -209,50 +209,29 @@ with ceval_CEval (fuel : nat) :
   forall {c : Com} {s1 s2 : State},
     ceval fuel c s1 = Some s2 -> CEval c s1 s2.
 Proof.
-  destruct fuel as [| fuel']; cbn; intros.
-    inv H.
-    destruct a.
-      1-2: inv H.
-      destruct (aeval fuel' a1 s) eqn: H1,
-               (aeval fuel' a2 s) eqn: H2; inv H; eauto.
-      destruct (aeval fuel' a1 s) eqn: H1,
-               (aeval fuel' a2 s) eqn: H2; inv H; eauto.
-      destruct (aeval fuel' a1 s) eqn: H1,
-               (aeval fuel' a2 s) eqn: H2; inv H; eauto.
-      destruct (ceval fuel' c s) eqn: H1; inv H; eauto.
-  destruct fuel as [| fuel']; cbn; intros.
-    inv H.
-    destruct e.
-      1-2: inv H; auto.
-      destruct (aeval fuel' a s) eqn: H1,
-               (aeval fuel' a0 s) eqn: H2; inv H; eauto.
-      destruct (aeval fuel' a s) eqn: H1,
-               (aeval fuel' a0 s) eqn: H2; inv H; eauto.
-      destruct (beval fuel' e s) eqn: H1; inv H; eauto.
-      destruct (beval fuel' e1 s) eqn: H1,
-               (beval fuel' e2 s) eqn: H2; inv H; eauto.
-      destruct (beval fuel' e1 s) eqn: H1,
-               (beval fuel' e2 s) eqn: H2; inv H; eauto.
-  destruct fuel as [| fuel']; cbn; intros.
-    inv H.
+  - destruct fuel as [| fuel']; cbn; intros.
+    + easy.
+    + destruct a; [now inv H | now inv H |
+        now destruct (aeval fuel' a1 s) eqn: H1, (aeval fuel' a2 s) eqn: H2; inv H; eauto.. |].
+      now destruct (ceval fuel' c s) eqn: H1; inv H; eauto.
+  - destruct fuel as [| fuel']; cbn; intros.
+    + easy.
+    + destruct e.
+      * now inv H.
+      * now inv H.
+      * now destruct (aeval fuel' a s) eqn: H1, (aeval fuel' a0 s) eqn: H2; inv H; eauto.
+      * now destruct (aeval fuel' a s) eqn: H1, (aeval fuel' a0 s) eqn: H2; inv H; eauto.
+      * now destruct (beval fuel' e s) eqn: H1; inv H; eauto.
+      * now destruct (beval fuel' e1 s) eqn: H1, (beval fuel' e2 s) eqn: H2; inv H; eauto.
+      * now destruct (beval fuel' e1 s) eqn: H1, (beval fuel' e2 s) eqn: H2; inv H; eauto.
+  - destruct fuel as [| fuel']; cbn; intros; [easy |].
     destruct c.
-      inv H.
-      destruct (aeval fuel' a s1) eqn: H1; inv H; eauto.
-      destruct (ceval fuel' c1 s1) eqn: H1; inv H; eauto.
-      destruct (beval fuel' b s1) eqn: H1.
-        destruct b0; eauto.
-        inv H.
-      destruct (beval fuel' b s1) eqn: H1; inv H.
-        destruct b0; inv H2; eauto.
-        destruct (ceval fuel' c s1) eqn: H; inv H0; eauto.
+    * now inversion H; subst; constructor.
+    * now destruct (aeval fuel' a s1) eqn: H1; inv H; eauto.
+    * now destruct (ceval fuel' c1 s1) eqn: H1; inv H; eauto.
+    * destruct (beval fuel' b s1) eqn: H1; [| easy].
+      now destruct b0; eauto.
+    * destruct (beval fuel' b s1) eqn: H1; [| easy].
+      destruct b0; inv H; eauto.
+      now destruct (ceval fuel' c s1) eqn: H'; inv H1; eauto.
 Qed.
-
-(*
-Lemma AEval_aeval :
-  forall {fuel : nat} {a : AExp} {s : State} {n : nat},
-    AEval a s n -> aeval fuel a s = n
-
-with BEval_beval :
-  forall {n : nat} {e : BExp} {s : State} {b : bool},
-    BEval e s b -> beval n e s = b
-*)
